examples/linked-lists/rev_why.v
@@ -64,7 +64,12 @@ Absurd r0=null; Intuition.
 Exists (cons r0 x); Exists l; Subst; Intuition.
 Apply List_of_cons; Intuition.
 Unfold access_pointer; Unfold 2 update_pointer.
-Rewrite pupdate_paccess_same.
+Rewrite pupdate_paccess_same; Auto.
+Apply list_of_update_same; Auto.
+Unfold disjoint in H1; Intuition.
+Apply (H7 r0); Auto.
+Rewrite <- H6; Auto with *.
+Apply list_of_update_same; Auto.
 
 
 Save.
@@ -129,28 +134,6 @@ Rewrite pupdate_paccess_same.
 Apply is_valid_update.
 Save.
 
-Proof.
-Magic.
-(* FILL PROOF HERE *)
-Save.
-
-Proof.
-Magic.
-(* FILL PROOF HERE *)
-Save.
-
-Proof.
-Magic.
-(* FILL PROOF HERE *)
-Save.
-
-Proof.
-Destruct result2; Intuition.
-Save.
-
-Proof.
-Destruct result2; Intuition.
-Save.
 
 Proof.
 Intuition.
@@ -166,11 +149,29 @@ Inversion Pre2; Intuition.
 Absurd p1=null; Auto.
 Save.
 
-Proof.
-Intros; Rewrite Pre3; Intuition.
-Save.
 
+(* Why obligation from file "rev.mlw", characters 1690-1692 *)
+Lemma rev_po_5 : 
+  (p0: pointer)
+  (Ltl: pointer_store)
+  (Pre4: (EX l:plist | (list_of Ltl p0 l)))
+  (result: pointer)
+  (Post8: result = p0)
+  (result0: pointer)
+  (Post7: result0 = result)
+  (p1: pointer)
+  (Post1: p1 = null)
+  (Ltl0: pointer_store)
+  (p2: pointer)
+  (r0: pointer)
+  (Post6: (EX lp:plist |
+           (EX lr:plist | (list_of Ltl0 p2 lp) /\ (list_of Ltl0 r0 lr) /\
+            (disjoint lp lr) /\
+            ((l:plist) ((list_of Ltl0 p0 l) -> (app (rev lr) lp) = (rev l))))) /\
+          r0 = null)
+  (EX l:plist | (list_of Ltl0 p2 l) /\
+   ((l0:plist) ((list_of Ltl0 p0 l0) -> l = (rev l0)))).
 Proof.
-Intros; Subst result; Intuition.
+(* FILL PROOF HERE *)
 Save.
 
